\documentclass{article}
\usepackage{amsmath}
\usepackage{amsthm}
\usepackage{hyperref}

\newtheorem{theorem}{Theorem}

\author{Arthur Allshire}
\title{A Programmer's Introduction to Mathematics: Chapter 2 Exercise solutions}
\begin{document}
\maketitle

\section*{2.6: Prove Vieta's Formulas}
{\it Exercise.} Let $f(x) = a_0 + a_1x + ... + a_nx^n$ be a degree $n$ polynomial, and suppose
it has $k$ real roots $r_1, ..., r_n$. Prove Vieta's Formulas, which are

\[
\begin{aligned}
\displaystyle\sum_{i=1}^{n} r_i = -\frac{a_{n-1}}{a_n}
\end{aligned}
\]

\[
\begin{aligned}
\displaystyle\prod_{i=1}^{n} r_i = (-1)^n \frac{a_0}{a_n}.
\end{aligned}
\]

\begin{proof}

Let $g(x) = \frac{f(x)}{a_n} = \frac{a_0}{a_n} + \frac{a_1}{a_n}x + ... + x^n$.
Now, given roots of $g(x)$ are $r_1,...,r_n$, the monic polynomial

\[
\begin{aligned}
g(x) = \displaystyle\prod_{i=1}^{n} x_i - r_i = \displaystyle\sum_{i=0}^{n} \frac{a_i}{a_n} x_i
\end{aligned}
\]
Now, \href{https://en.wikipedia.org/wiki/Equating_coefficients}{equating the coefficients}
of $a^n-1$ an both sides (observe the expansion of the product on the left hand side resulting in
the multiplication of $r_i$ by $x$ $n-1$ times), we get
\[
\begin{aligned}
\displaystyle\sum_{i=1}^{n} r_i = -\frac{a_{n-1}}{a_n}
\end{aligned},
\]as required.
Similarly, we simply observe equate the constant term (the "coefficient of $x^0$") on both sides,
observing that on the left hand side this is the product of the roots multiplied by $(-1)^n$, and
divide through by $(-1)^n$ to obtain the second equation.

\end{proof}

\end{document}
